---
layout: post
title:  "TIL-Fast Fibonacci"
summary: TIL journal
author: JHJ
date: '2022-02-15'
category: TIL
keywords: Algorithm
usemathjax: true
--- 

# Fast Fibonacci
## Finding Nth fibonacci number using Matrix exponentiation and binary power operation 
<br>  

### 1. Fibonacci Sequence as matrix operation  
-  Nth fibonacci number  
$$ F(N) = F(N-1) + F(N-2)$$

- Using matrix multipication
$$ 
\begin{bmatrix}  F(N) \\ F(N-1) \end{bmatrix}
=
 \begin{bmatrix}  1 & 1 \\ 1 & 0 \end{bmatrix}
\begin{bmatrix}  F(N-1) \\ F(N-2) \end{bmatrix} 
$$

- More example _F(4)_
$$
\begin{bmatrix}  F(4) \\ F(3) \end{bmatrix}
=
 \begin{bmatrix}  1 & 1 \\ 1 & 0 \end{bmatrix}
\begin{bmatrix}  F(3) \\ F(2) \end{bmatrix} 
$$

- F(3) is 
$$
\begin{bmatrix}  F(3) \\ F(2) \end{bmatrix}
=
 \begin{bmatrix}  1 & 1 \\ 1 & 0 \end{bmatrix}
\begin{bmatrix}  F(2) \\ F(1) \end{bmatrix} 
$$

- F(4) becomes
$$
\begin{bmatrix}  F(4) \\ F(3) \end{bmatrix}
=
 \begin{bmatrix}  1 & 1 \\ 1 & 0 \end{bmatrix}
 \begin{bmatrix}  1 & 1 \\ 1 & 0 \end{bmatrix}
\begin{bmatrix}  F(2) \\ F(1) \end{bmatrix} 
$$

- F(2) is
$$
\begin{bmatrix}  F(2) \\ F(1) \end{bmatrix}
=
 \begin{bmatrix}  1 & 1 \\ 1 & 0 \end{bmatrix}
\begin{bmatrix}  F(1) \\ F(0) \end{bmatrix} 
$$

- F(4) becomes
$$
\begin{bmatrix}  F(4) \\ F(3) \end{bmatrix}
=
 \begin{bmatrix}  1 & 1 \\ 1 & 0 \end{bmatrix}
 \begin{bmatrix}  1 & 1 \\ 1 & 0 \end{bmatrix}
 \begin{bmatrix}  1 & 1 \\ 1 & 0 \end{bmatrix}
\begin{bmatrix}  F(1) \\ F(0) \end{bmatrix} 
$$

- Base F(1) = 1, and F(2) = 0
$$
\begin{bmatrix}  F(4) \\ F(3) \end{bmatrix}
=
 \begin{bmatrix}  1 & 1 \\ 1 & 0 \end{bmatrix}
 \begin{bmatrix}  1 & 1 \\ 1 & 0 \end{bmatrix}
 \begin{bmatrix}  1 & 1 \\ 1 & 0 \end{bmatrix}
\begin{bmatrix}  1 \\ 0 \end{bmatrix} 
$$

$$
\begin{bmatrix}  F(4) \\ F(3) \end{bmatrix}
=
 \begin{bmatrix}  1 & 1 \\ 1 & 0 \end{bmatrix}^{3}
\begin{bmatrix}  1 \\ 0 \end{bmatrix} 
$$

- Finally, General equation is
$$
\begin{bmatrix}  F(N) \\ F(N-1) \end{bmatrix}
=
 \begin{bmatrix}  1 & 1 \\ 1 & 0 \end{bmatrix}^{N-1}
\begin{bmatrix}  1 \\ 0 \end{bmatrix} 
$$

- Let
$$
 \begin{bmatrix}  1 & 1 \\ 1 & 0 \end{bmatrix}^{N-1}
=
 \begin{bmatrix}  a & b \\ c & d \end{bmatrix}
$$

- Then, F(N) is
$$ F(N) = a$$
### 2. Binary Exponentiation
This is better explained by an example.
$$ 3^{25} = 3^{2^4 + 2^3 + 2^0} $$

<pre>
ans = 1
At each step a = a * a

1. 11001
       ^
Bit is on -> ans = ans * a
    ans = a
    a *= a => a^2

2. 11001
      ^
Bit is off 
    ans = a
    a^2 *= a^2 => a^4

1. 11001
     ^
Bit is off
    ans = 1
    a^4 *= a^4 => a^8

4. 11001
    ^
Bit is on -> ans = ans * a^8
    ans = ans(a) * a^8 => a^9
    a^8 *= a^8 =>a^16

5. 11001
   ^
Bit is on -> ans = ans * a^16
    ans = ans(a^9) * a^16 => a^25
</pre>
- Code Implementation (in c++)
```c++
int binaryPower(int a, int n)
{
    int ans = 1;
    while (n)
    {
        if (n&1)
            ans = ans * a;
        a *= a;
        n = n >> 1; 
    }
    return ans;
}
```   
<br>  

### 3. Final Implementation(in Python)
```python
def matrixMul(m1, m2):
    # 4x4 matrix multiplication
    a11 = m1[0][0]
    a12 = m1[0][1]
    a21 = m1[1][0]
    a22 = m1[1][1]
    
    b11 = m2[0][0]
    b12 = m2[0][1]
    b21 = m2[1][0]
    b22 = m2[1][1]

    m1[0][0] = a11*b11 + a12*b21
    m1[0][1] = a11*b12 + a12*b22
    m1[1][0] = a21*b11 + a22*b21
    m1[1][1] = a21*b12 + a22*b22

def powerMat(n):
	M = [[1, 1], [1, 0]]
	ans = [[1, 0], [0, 1]]

	# binary exponentiation
	while n > 0:
		if n & 1:
			matrixMul(ans, M)
		matrixMul(M, M)
		n = n >> 1

	return ans[0][0]

def solution(x):
	return powerMat(x-1)

```

  